ironfleet/src/Dafny/Distributed/Concur/Reduction3.i.dfy
@@ -6,7 +6,254 @@ module Reduction3Module
     import opened Reduction2Module
     import opened Collections__Seqs_i
 
-    lemma lemma_PerformReductionOfSpecificIndicesHelper1(
+    lemma {:timeLimitMultiplier 2} lemma_PerformReductionOfSpecificIndicesHelper1(
+        trace:Trace,
+        trace':Trace,
+        min_level:int,
+        max_level:int,
+        group:seq<Entry>,
+        indices:seq<int>,
+        indices':seq<int>,
+        updated_index:int,
+        cur_pos:int,
+        desired_pos:int
+        )
+        requires TraceValid(trace, min_level, max_level);
+        requires min_level < max_level;
+        requires |indices| == |group| > 0;
+        requires forall i, j {:trigger indices[i], indices[j]} :: 0 <= i < j < |indices| ==> indices[i] < indices[j];
+        requires forall i :: 0 <= i < |indices| ==> 0 <= indices[i] < |trace| && trace[indices[i]] == group[i];
+        requires 0 <= updated_index < |indices|-1;
+        requires forall i, trace_index {:trigger indices[i], trace[trace_index], indices[i+1]} ::
+                                      0 <= i < |indices| - 1
+                                   && indices[i] < trace_index < indices[i+1]
+                                   ==> GetEntryActor(trace[trace_index]) != GetEntryActor(group[0]);
+        requires GetEntryActor(group[0]) == GetEntryActor(trace[indices[updated_index]]);
+        requires indices' == indices[updated_index := indices[updated_index+1]-1]
+        requires cur_pos == indices[updated_index];
+        requires desired_pos == indices[updated_index+1]-1;
+        requires cur_pos <= desired_pos;
+        requires trace' == MoveTraceElementRight(trace, cur_pos, desired_pos);
+        ensures  TraceValid(trace', min_level, max_level);
+        ensures  forall i, trace_index {:trigger indices'[i], trace'[trace_index], indices'[i+1]} ::
+                                      0 <= i < |indices'| - 1
+                                   && indices'[i] < trace_index < indices'[i+1]
+                                   ==> GetEntryActor(trace'[trace_index]) != GetEntryActor(group[0]);
+    {
+        forall actor:Actor
+            ensures ActorTraceValid(RestrictTraceToActor(trace', actor), min_level, max_level);
+        {
+            var actor_trace := RestrictTraceToActor(trace, actor);
+            var actor_trace' := RestrictTraceToActor(trace', actor);
+
+            var second_component := trace[cur_pos+1..desired_pos+1];
+            var third_component := [trace[cur_pos]];
+
+            if actor == GetEntryActor(group[0]) {
+                forall i | 0 <= i < |second_component|
+                    ensures GetEntryActor(second_component[i]) != actor;
+                {
+                    var j := i + cur_pos+1;
+                    assert second_component[i] == trace[j];
+                    assert indices[updated_index] < j < indices[updated_index+1];
+                    assert GetEntryActor(trace[j]) != actor;
+                }
+                lemma_RestrictTraceToActorEmpty(second_component, actor);
+            }
+            else {
+                lemma_RestrictTraceToActorEmpty(third_component, actor);
+            }
+
+            // Since one of the components' RestrictTraceToActor is empty, the two RestrictTraceToActors must commute.
+            assert RestrictTraceToActor(second_component, actor) + RestrictTraceToActor(third_component, actor) == RestrictTraceToActor(third_component, actor) + RestrictTraceToActor(second_component, actor);
+            assert RestrictTraceToActor(trace[cur_pos+1..desired_pos+1], actor) + RestrictTraceToActor([trace[cur_pos]], actor) ==
+                   RestrictTraceToActor([trace[cur_pos]], actor) + RestrictTraceToActor(trace[cur_pos+1..desired_pos+1], actor);
+
+            calc {
+                actor_trace';
+                RestrictTraceToActor(trace', actor);
+                RestrictTraceToActor(trace[..cur_pos] + trace[cur_pos+1..desired_pos+1] + [trace[cur_pos]] + trace[desired_pos+1..], actor);
+                    { lemma_Split4RestrictTraceToActor(trace[..cur_pos], trace[cur_pos+1..desired_pos+1], [trace[cur_pos]], trace[desired_pos+1..], actor); }
+                RestrictTraceToActor(trace[..cur_pos], actor) + RestrictTraceToActor(trace[cur_pos+1..desired_pos+1], actor) + RestrictTraceToActor([trace[cur_pos]], actor) + RestrictTraceToActor(trace[desired_pos+1..], actor);
+                RestrictTraceToActor(trace[..cur_pos], actor) + (RestrictTraceToActor(trace[cur_pos+1..desired_pos+1], actor) + RestrictTraceToActor([trace[cur_pos]], actor)) + RestrictTraceToActor(trace[desired_pos+1..], actor);
+                RestrictTraceToActor(trace[..cur_pos], actor) + (RestrictTraceToActor([trace[cur_pos]], actor) + RestrictTraceToActor(trace[cur_pos+1..desired_pos+1], actor)) + RestrictTraceToActor(trace[desired_pos+1..], actor);
+                    { assert RestrictTraceToActor(trace[..cur_pos], actor) + (RestrictTraceToActor([trace[cur_pos]], actor) + RestrictTraceToActor(trace[cur_pos+1..desired_pos+1], actor)) ==
+                             RestrictTraceToActor(trace[..cur_pos], actor) + RestrictTraceToActor([trace[cur_pos]], actor) + RestrictTraceToActor(trace[cur_pos+1..desired_pos+1], actor); }
+                RestrictTraceToActor(trace[..cur_pos], actor) + RestrictTraceToActor([trace[cur_pos]], actor) + RestrictTraceToActor(trace[cur_pos+1..desired_pos+1], actor) + RestrictTraceToActor(trace[desired_pos+1..], actor);
+                    { lemma_Split4RestrictTraceToActor(trace[..cur_pos], [trace[cur_pos]], trace[cur_pos+1..desired_pos+1], trace[desired_pos+1..], actor); }
+                RestrictTraceToActor(trace[..cur_pos] + [trace[cur_pos]] + trace[cur_pos+1..desired_pos+1] + trace[desired_pos+1..], actor);
+                    { assert trace[..cur_pos+1] == trace[..cur_pos] + [trace[cur_pos]]; }
+                RestrictTraceToActor(trace[..cur_pos+1] + trace[cur_pos+1..desired_pos+1] + trace[desired_pos+1..], actor);
+                    { assert trace[..cur_pos+1] + trace[cur_pos+1..desired_pos+1] == trace[..desired_pos+1]; }
+                RestrictTraceToActor(trace[..desired_pos+1] + trace[desired_pos+1..], actor);
+                    { assert trace[..desired_pos+1] + trace[desired_pos+1..] == trace; }
+                RestrictTraceToActor(trace, actor);
+                actor_trace;
+            }
+        }
+        assert TraceValid(trace', min_level, max_level);
+    }
+
+    lemma lemma_PerformReductionOfSpecificIndicesHelper2(
+        trace:Trace,
+        trace':Trace,
+        entry_pos:int,
+        cur_pos:int,
+        desired_pos:int
+        )
+        requires 0 <= entry_pos <= cur_pos <= desired_pos < |trace|;
+        requires trace' == MoveTraceElementRight(trace, cur_pos, desired_pos);
+        ensures  trace'[..entry_pos] == trace[..entry_pos];
+    {
+        assert |trace'[..entry_pos]| == entry_pos == |trace[..entry_pos]|;
+        forall i | 0 <= i < |trace'[..entry_pos]|
+            ensures trace'[..entry_pos][i] == trace[..entry_pos][i];
+        {
+            calc {
+                trace'[..entry_pos][i];
+                trace'[i];
+                    { assert i < cur_pos; }
+                trace[i];
+                trace[..entry_pos][i];
+            }
+        }
+    }
+
+    lemma {:timeLimitMultiplier 2} lemma_PerformReductionOfSpecificIndicesHelper3(
+        trace:Trace,
+        trace':Trace,
+        min_level:int,
+        max_level:int,
+        group:seq<Entry>,
+        indices:seq<int>,
+        indices':seq<int>,
+        updated_index:int,
+        cur_pos:int,
+        desired_pos:int
+        )
+        requires TraceValid(trace, min_level, max_level);
+        requires min_level < max_level;
+        requires |indices| == |group| > 0;
+        requires forall i, j {:trigger indices[i], indices[j]} :: 0 <= i < j < |indices| ==> indices[i] < indices[j];
+        requires forall i :: 0 <= i < |indices| ==> 0 <= indices[i] < |trace| && trace[indices[i]] == group[i];
+        requires 0 < updated_index < |indices|;
+        requires forall i, trace_index {:trigger indices[i], trace[trace_index], indices[i+1]} ::
+                                      0 <= i < |indices| - 1
+                                   && indices[i] < trace_index < indices[i+1]
+                                   ==> GetEntryActor(trace[trace_index]) != GetEntryActor(group[0]);
+        requires GetEntryActor(group[0]) == GetEntryActor(trace[indices[updated_index]]);
+        requires indices' == indices[updated_index := indices[updated_index-1]+1];
+        requires cur_pos == indices[updated_index];
+        requires desired_pos == indices[updated_index-1]+1;
+        requires desired_pos <= cur_pos;
+        requires trace' == MoveTraceElementLeft(trace, cur_pos, desired_pos);
+        ensures  TraceValid(trace', min_level, max_level);
+        ensures  forall i, trace_index {:trigger indices'[i], trace'[trace_index], indices'[i+1]} ::
+                                      0 <= i < |indices'| - 1
+                                   && indices'[i] < trace_index < indices'[i+1]
+                                   ==> GetEntryActor(trace'[trace_index]) != GetEntryActor(group[0]);
+    {
+        forall actor:Actor
+            ensures ActorTraceValid(RestrictTraceToActor(trace', actor), min_level, max_level);
+        {
+            var actor_trace := RestrictTraceToActor(trace, actor);
+            var actor_trace' := RestrictTraceToActor(trace', actor);
+
+            var second_component := [trace[cur_pos]];
+            var third_component := trace[desired_pos..cur_pos];
+
+            if actor == GetEntryActor(group[0]) {
+                forall i | 0 <= i < |third_component|
+                    ensures GetEntryActor(third_component[i]) != actor;
+                {
+                    var j := i + desired_pos;
+                    assert third_component[i] == trace[j];
+                    assert indices[updated_index-1] < j < indices[updated_index-1+1];
+                    assert GetEntryActor(trace[j]) != actor;
+                }
+                lemma_RestrictTraceToActorEmpty(third_component, actor);
+            }
+            else {
+                lemma_RestrictTraceToActorEmpty(second_component, actor);
+            }
+
+            // Since one of the components' RestrictTraceToActor is empty, the two RestrictTraceToActors must commute.
+            assert RestrictTraceToActor(second_component, actor) + RestrictTraceToActor(third_component, actor) == RestrictTraceToActor(third_component, actor) + RestrictTraceToActor(second_component, actor);
+            assert RestrictTraceToActor(trace[desired_pos..cur_pos], actor) + RestrictTraceToActor([trace[cur_pos]], actor) ==
+                   RestrictTraceToActor([trace[cur_pos]], actor) + RestrictTraceToActor(trace[desired_pos..cur_pos], actor);
+
+            calc {
+                actor_trace';
+                RestrictTraceToActor(trace', actor);
+                RestrictTraceToActor(trace[..desired_pos] + [trace[cur_pos]] + trace[desired_pos..cur_pos] + trace[cur_pos+1..], actor);
+                    { lemma_Split4RestrictTraceToActor(trace[..desired_pos], [trace[cur_pos]], trace[desired_pos..cur_pos], trace[cur_pos+1..], actor); }
+                RestrictTraceToActor(trace[..desired_pos], actor) + RestrictTraceToActor([trace[cur_pos]], actor) + RestrictTraceToActor(trace[desired_pos..cur_pos], actor) + RestrictTraceToActor(trace[cur_pos+1..], actor);
+                RestrictTraceToActor(trace[..desired_pos], actor) + (RestrictTraceToActor([trace[cur_pos]], actor) + RestrictTraceToActor(trace[desired_pos..cur_pos], actor)) + RestrictTraceToActor(trace[cur_pos+1..], actor);
+                RestrictTraceToActor(trace[..desired_pos], actor) + (RestrictTraceToActor(trace[desired_pos..cur_pos], actor) + RestrictTraceToActor([trace[cur_pos]], actor)) + RestrictTraceToActor(trace[cur_pos+1..], actor);
+                RestrictTraceToActor(trace[..desired_pos], actor) + RestrictTraceToActor(trace[desired_pos..cur_pos], actor) + RestrictTraceToActor([trace[cur_pos]], actor) + RestrictTraceToActor(trace[cur_pos+1..], actor);
+                    { lemma_Split4RestrictTraceToActor(trace[..desired_pos], trace[desired_pos..cur_pos], [trace[cur_pos]], trace[cur_pos+1..], actor); }
+                RestrictTraceToActor(trace[..desired_pos] + trace[desired_pos..cur_pos] + [trace[cur_pos]] + trace[cur_pos+1..], actor);
+                    { assert trace[..cur_pos] == trace[..desired_pos] + trace[desired_pos..cur_pos]; }
+                RestrictTraceToActor(trace[..cur_pos] + [trace[cur_pos]] + trace[cur_pos+1..], actor);
+                    { assert trace[..cur_pos] + [trace[cur_pos]] == trace[..cur_pos+1]; }
+                RestrictTraceToActor(trace[..cur_pos+1] + trace[cur_pos+1..], actor);
+                    { assert trace[..cur_pos+1] + trace[cur_pos+1..] == trace; }
+                RestrictTraceToActor(trace, actor);
+                actor_trace;
+            }
+        }
+        assert TraceValid(trace', min_level, max_level);
+
+        forall i, trace_index {:trigger indices'[i], trace'[trace_index], indices'[i+1]} |
+                                      0 <= i < |indices'| - 1
+                                   && indices'[i] < trace_index < indices'[i+1]
+            ensures GetEntryActor(trace'[trace_index]) != GetEntryActor(group[0]);
+        {
+            if i < updated_index-1 {
+            }
+            else if i == updated_index-1 {
+            }
+            else if i == updated_index {
+                if trace_index > indices[updated_index] {
+                }
+                else {
+                    assert indices'[updated_index] < trace_index <= indices[updated_index];
+                    assert indices[updated_index-1]+1 < trace_index <= indices[updated_index];
+                    assert indices[updated_index-1]+1 < trace_index <= indices[updated_index-1+1];
+                    assert GetEntryActor(trace'[trace_index]) != GetEntryActor(group[0]);
+                }
+            }
+            else {
+            }
+        }
+    }
+
+    lemma lemma_PerformReductionOfSpecificIndicesHelper4(
+        trace:Trace,
+        trace':Trace,
+        entry_pos:int,
+        cur_pos:int,
+        desired_pos:int
+        )
+        requires 0 <= entry_pos <= desired_pos <= cur_pos < |trace|;
+        requires trace' == MoveTraceElementLeft(trace, cur_pos, desired_pos);
+        ensures  trace'[..entry_pos] == trace[..entry_pos];
+    {
+        assert |trace'[..entry_pos]| == entry_pos == |trace[..entry_pos]|;
+        forall i | 0 <= i < |trace'[..entry_pos]|
+            ensures trace'[..entry_pos][i] == trace[..entry_pos][i];
+        {
+            calc {
+                trace'[..entry_pos][i];
+                trace'[i];
+                    { assert i < cur_pos; }
+                trace[i];
+                trace[..entry_pos][i];
+            }
+        }
+    }
+
+    lemma lemma_PerformReductionOfSpecificIndicesHelper5(
         trace:Trace,
         min_level:int,
         mid_level:int,
@@ -21,7 +268,7 @@ module Reduction3Module
         requires TraceValid(trace, min_level, max_level);
         requires |indices| == |group| > 0;
         requires 0 <= entry_pos <= indices[0];
-        requires forall i, j {:trigger indices[i] < indices[j]}{:trigger indices[i] <= indices[j]}{:trigger indices[j] > indices[i]}{:trigger indices[j] >= indices[i]} :: 0 <= i < j < |indices| ==> indices[i] < indices[j];
+        requires forall i, j {:trigger indices[i], indices[j]} :: 0 <= i < j < |indices| ==> indices[i] < indices[j];
         requires forall i :: 0 <= i < |indices| ==> 0 <= indices[i] < |trace| && trace[indices[i]] == group[i];
         requires min_level < mid_level <= max_level;
         requires EntryGroupValidForLevels(group, min_level, mid_level);
@@ -63,7 +310,7 @@ module Reduction3Module
         assert group == group_alt;
     }
 
-    lemma lemma_PerformReductionOfSpecificIndicesHelper2(
+    lemma lemma_PerformReductionOfSpecificIndicesHelper6(
         trace:Trace,
         min_level:int,
         mid_level:int,
@@ -129,7 +376,7 @@ module Reduction3Module
         }
     }
 
-    lemma lemma_PerformReductionOfSpecificIndicesHelper3(
+    lemma lemma_PerformReductionOfSpecificIndicesHelper7(
         trace:Trace,
         min_level:int,
         mid_level:int,
@@ -195,6 +442,271 @@ module Reduction3Module
         }
     }
 
+    lemma {:timeLimitMultiplier 4} lemma_PerformReductionOfSpecificIndicesCase1(
+        trace:Trace,
+        db:seq<DistributedSystemState>,
+        min_level:int,
+        mid_level:int,
+        max_level:int,
+        entry_pos:int,
+        indices:seq<int>,
+        group:seq<Entry>,
+        pivot_index:int,
+        in_position_left:int,
+        in_position_right:int
+        ) returns (
+        trace':Trace,
+        db':seq<DistributedSystemState>
+        )
+        requires IsValidDistributedSystemTraceAndBehavior(trace, db);
+        requires TraceValid(trace, min_level, max_level);
+        requires |indices| == |group| > 0;
+        requires 0 <= entry_pos <= indices[0];
+        requires forall i, j {:trigger indices[i], indices[j]} :: 0 <= i < j < |indices| ==> indices[i] < indices[j];
+        requires forall i :: 0 <= i < |indices| ==> 0 <= indices[i] < |trace| && trace[indices[i]] == group[i];
+        requires min_level < mid_level <= max_level;
+        requires EntryGroupValidForLevels(group, min_level, mid_level);
+        requires GetEntryLevel(group[0]) == min_level;
+        requires pivot_index == last(group).pivot_index;
+        requires forall i :: 0 <= i < |group| ==> GetEntryActor(group[i]) == GetEntryActor(group[0]);   // All for the same actor
+        requires forall i, trace_index {:trigger indices[i], trace[trace_index], indices[i+1]} ::
+                                      0 <= i < |indices| - 1
+                                   && indices[i] < trace_index < indices[i+1]
+                                   ==> GetEntryActor(trace[trace_index]) != GetEntryActor(group[0]);
+        requires 0 < in_position_left <= pivot_index <= in_position_right < |group|;
+        requires forall k :: in_position_left <= k <= in_position_right ==> k - pivot_index == indices[k] - indices[pivot_index];
+
+        ensures  TraceValid(trace', min_level, max_level);
+        ensures  IsValidDistributedSystemTraceAndBehavior(trace', db');
+        ensures  DistributedSystemBehaviorRefinesSpec(db')
+                 ==> exists sb :: DistributedSystemBehaviorRefinesSpecBehaviorWithNonPivotsAsStutters(db, sb, indices, pivot_index);
+        ensures  entry_pos <= |trace'| < |trace|;
+        ensures  trace'[..entry_pos] == trace[..entry_pos];
+        decreases |group| - in_position_right + in_position_left, 0;
+    {
+        var actor := GetEntryActor(group[0]);
+
+        assert indices[in_position_left-1] < indices[in_position_left];
+        forall trace_index | indices[in_position_left-1] < trace_index <= indices[in_position_left]-1
+            ensures GetEntryActor(trace[trace_index]) != GetEntryActor(trace[indices[in_position_left-1]]);
+        {
+            var j := in_position_left-1;
+            assert indices[j] < trace_index < indices[j+1];
+        }
+
+        var cur_pos := indices[in_position_left-1];
+        var desired_pos := indices[in_position_left]-1;
+        var trace_mid, db_mid := lemma_MoveRightMoverIntoPlace(trace, db, cur_pos, desired_pos);
+        var indices_mid := indices[in_position_left-1 := indices[in_position_left]-1];
+
+        lemma_PerformReductionOfSpecificIndicesHelper1(trace, trace_mid, min_level, max_level, group, indices, indices_mid, in_position_left-1, cur_pos, desired_pos);
+        trace', db' := lemma_PerformReductionOfSpecificIndices(trace_mid, db_mid, min_level, mid_level, max_level, entry_pos, indices_mid, group, pivot_index, in_position_left - 1, in_position_right);
+
+        if DistributedSystemBehaviorRefinesSpec(db') {
+            var sb' :| DistributedSystemBehaviorRefinesSpecBehavior(db', sb');
+            var sb_mid :| DistributedSystemBehaviorRefinesSpecBehaviorWithNonPivotsAsStutters(db_mid, sb_mid, indices_mid, pivot_index);
+            assert DistributedSystemBehaviorRefinesSpecBehavior(db_mid, sb_mid);
+            assert sb_mid[desired_pos] == sb_mid[desired_pos+1];
+            var sb := ShiftSpecBehaviorSliceRight(sb_mid, cur_pos, desired_pos);
+            assert DistributedSystemBehaviorRefinesSpecBehavior(db, sb);
+            forall i | 0 <= i < |indices| && i != pivot_index
+                ensures 0 <= indices[i];
+                ensures indices[i] < |sb|-1;
+                ensures sb[indices[i]] == sb[indices[i] + 1];
+            {
+                if i < in_position_left - 1 {
+                    assert indices[i] < indices[in_position_left-1] == cur_pos;
+                    assert indices[i]+1 <= cur_pos;
+                    assert sb[indices[i]] == sb_mid[indices[i]];
+                    assert sb[indices[i]+1] == sb_mid[indices[i]+1];
+                    assert sb[indices[i]] == sb[indices[i] + 1];
+                }
+                else if i == in_position_left - 1 {
+                    assert sb[indices[i]] == sb[indices[i] + 1];
+                }
+                else if i == in_position_left {
+                    assert indices[i] == indices[in_position_left] == desired_pos + 1;
+                    assert sb[indices[i]] == sb_mid[indices[i]-1] == sb_mid[desired_pos];
+                    assert indices[i] + 1 > desired_pos + 1;
+                    assert sb[indices[i]+1] == sb_mid[indices[i]+1] == sb_mid[desired_pos+2];
+                }
+                else {
+                    assert indices[i] > indices[in_position_left];
+                    assert indices[i] > desired_pos + 1;
+                    assert sb[indices[i]] == sb_mid[indices[i]];
+                    assert sb[indices[i]+1] == sb_mid[indices[i]+1];
+                    assert sb[indices[i]] == sb[indices[i] + 1];
+                }
+            }
+            assert DistributedSystemBehaviorRefinesSpecBehaviorWithNonPivotsAsStutters(db, sb, indices, pivot_index);
+        }
+
+        lemma_PerformReductionOfSpecificIndicesHelper2(trace, trace_mid, entry_pos, cur_pos, desired_pos);
+    }
+
+    lemma lemma_PerformReductionOfSpecificIndicesCase2(
+        trace:Trace,
+        db:seq<DistributedSystemState>,
+        min_level:int,
+        mid_level:int,
+        max_level:int,
+        entry_pos:int,
+        indices:seq<int>,
+        group:seq<Entry>,
+        pivot_index:int,
+        in_position_left:int,
+        in_position_right:int
+        ) returns (
+        trace':Trace,
+        db':seq<DistributedSystemState>
+        )
+        requires IsValidDistributedSystemTraceAndBehavior(trace, db);
+        requires TraceValid(trace, min_level, max_level);
+        requires |indices| == |group| > 0;
+        requires 0 <= entry_pos <= indices[0];
+        requires forall i, j {:trigger indices[i], indices[j]} :: 0 <= i < j < |indices| ==> indices[i] < indices[j];
+        requires forall i :: 0 <= i < |indices| ==> 0 <= indices[i] < |trace| && trace[indices[i]] == group[i];
+        requires min_level < mid_level <= max_level;
+        requires EntryGroupValidForLevels(group, min_level, mid_level);
+        requires GetEntryLevel(group[0]) == min_level;
+        requires pivot_index == last(group).pivot_index;
+        requires forall i :: 0 <= i < |group| ==> GetEntryActor(group[i]) == GetEntryActor(group[0]);   // All for the same actor
+        requires forall i, trace_index {:trigger indices[i], trace[trace_index], indices[i+1]} ::
+                                      0 <= i < |indices| - 1
+                                   && indices[i] < trace_index < indices[i+1]
+                                   ==> GetEntryActor(trace[trace_index]) != GetEntryActor(group[0]);
+        requires 0 == in_position_left <= pivot_index <= in_position_right < |group| - 1;
+        requires forall k :: in_position_left <= k <= in_position_right ==> k - pivot_index == indices[k] - indices[pivot_index];
+
+        ensures  TraceValid(trace', min_level, max_level);
+        ensures  IsValidDistributedSystemTraceAndBehavior(trace', db');
+        ensures  DistributedSystemBehaviorRefinesSpec(db')
+                 ==> exists sb :: DistributedSystemBehaviorRefinesSpecBehaviorWithNonPivotsAsStutters(db, sb, indices, pivot_index);
+        ensures  entry_pos <= |trace'| < |trace|;
+        ensures  trace'[..entry_pos] == trace[..entry_pos];
+        decreases |group| - in_position_right + in_position_left, 0;
+    {
+        var actor := GetEntryActor(group[0]);
+
+        assert indices[in_position_right+1] > indices[in_position_right];
+        forall trace_index | indices[in_position_right] < trace_index <= indices[in_position_right+1]-1
+            ensures GetEntryActor(trace[trace_index]) != GetEntryActor(trace[indices[in_position_right+1]]);
+        {
+        }
+
+        var cur_pos := indices[in_position_right+1];
+        var desired_pos := indices[in_position_right]+1;
+        var trace_mid, db_mid := lemma_MoveLeftMoverIntoPlace(trace, db, cur_pos, desired_pos);
+        var indices_mid := indices[in_position_right+1 := indices[in_position_right]+1];
+
+        lemma_PerformReductionOfSpecificIndicesHelper3(trace, trace_mid, min_level, max_level, group, indices, indices_mid, in_position_right+1, cur_pos, desired_pos);
+        trace', db' := lemma_PerformReductionOfSpecificIndices(trace_mid, db_mid, min_level, mid_level, max_level, entry_pos, indices_mid, group, pivot_index, in_position_left, in_position_right + 1);
+
+        if DistributedSystemBehaviorRefinesSpec(db') {
+            var sb' :| DistributedSystemBehaviorRefinesSpecBehavior(db', sb');
+            var sb_mid :| DistributedSystemBehaviorRefinesSpecBehaviorWithNonPivotsAsStutters(db_mid, sb_mid, indices_mid, pivot_index);
+            assert DistributedSystemBehaviorRefinesSpecBehavior(db_mid, sb_mid);
+            assert sb_mid[indices_mid[in_position_right+1]] == sb_mid[indices_mid[in_position_right+1]+1];
+            assert sb_mid[desired_pos] == sb_mid[desired_pos+1];
+            var sb := ShiftSpecBehaviorSliceLeft(sb_mid, cur_pos, desired_pos);
+            assert DistributedSystemBehaviorRefinesSpecBehavior(db, sb);
+            forall i | 0 <= i < |indices| && i != pivot_index
+                ensures 0 <= indices[i];
+                ensures indices[i] < |sb|-1;
+                ensures sb[indices[i]] == sb[indices[i] + 1];
+            {
+                if i < in_position_right {
+                    assert indices[i] < indices[in_position_right] == desired_pos - 1;
+                    assert indices[i]+1 <= desired_pos;
+                    assert sb[indices[i]] == sb_mid[indices[i]];
+                    assert sb[indices[i]+1] == sb_mid[indices[i]+1];
+                    assert sb[indices[i]] == sb[indices[i] + 1];
+                }
+                else if i == in_position_right {
+                    assert indices[i] == indices[in_position_right] == desired_pos - 1;
+                    assert sb[indices[i]] == sb_mid[indices[i]] == sb_mid[desired_pos-1];
+                    assert indices[i] + 1 == desired_pos;
+                    assert sb[indices[i]+1] == sb_mid[desired_pos] == sb_mid[desired_pos-1+1];
+                }
+                else if i == in_position_right + 1 {
+                    assert sb[indices[i]] == sb[indices[i] + 1];
+                }
+                else {
+                    assert indices[i] > indices[in_position_right+1];
+                    assert indices[i] > cur_pos;
+                    assert indices[i] >= cur_pos + 1;
+                    assert sb[indices[i]] == sb_mid[indices[i]];
+                    assert sb[indices[i]+1] == sb_mid[indices[i]+1];
+                    assert sb[indices[i]] == sb[indices[i] + 1];
+                }
+            }
+            assert DistributedSystemBehaviorRefinesSpecBehaviorWithNonPivotsAsStutters(db, sb, indices, pivot_index);
+        }
+
+        lemma_PerformReductionOfSpecificIndicesHelper4(trace, trace_mid, entry_pos, cur_pos, desired_pos);
+    }
+
+    lemma {:timeLimitMultiplier 2} lemma_PerformReductionOfSpecificIndicesCase3(
+        trace:Trace,
+        db:seq<DistributedSystemState>,
+        min_level:int,
+        mid_level:int,
+        max_level:int,
+        entry_pos:int,
+        indices:seq<int>,
+        group:seq<Entry>,
+        pivot_index:int,
+        in_position_left:int,
+        in_position_right:int
+        ) returns (
+        trace':Trace,
+        db':seq<DistributedSystemState>
+        )
+        requires IsValidDistributedSystemTraceAndBehavior(trace, db);
+        requires TraceValid(trace, min_level, max_level);
+        requires |indices| == |group| > 0;
+        requires 0 <= entry_pos <= indices[0];
+        requires forall i, j {:trigger indices[i], indices[j]} :: 0 <= i < j < |indices| ==> indices[i] < indices[j];
+        requires forall i :: 0 <= i < |indices| ==> 0 <= indices[i] < |trace| && trace[indices[i]] == group[i];
+        requires min_level < mid_level <= max_level;
+        requires EntryGroupValidForLevels(group, min_level, mid_level);
+        requires GetEntryLevel(group[0]) == min_level;
+        requires pivot_index == last(group).pivot_index;
+        requires forall i :: 0 <= i < |group| ==> GetEntryActor(group[i]) == GetEntryActor(group[0]);   // All for the same actor
+        requires forall i, trace_index {:trigger indices[i], trace[trace_index], indices[i+1]} ::
+                                      0 <= i < |indices| - 1
+                                   && indices[i] < trace_index < indices[i+1]
+                                   ==> GetEntryActor(trace[trace_index]) != GetEntryActor(group[0]);
+        requires 0 == in_position_left <= pivot_index <= in_position_right == |group| - 1;
+        requires forall k :: in_position_left <= k <= in_position_right ==> k - pivot_index == indices[k] - indices[pivot_index];
+
+        ensures  TraceValid(trace', min_level, max_level);
+        ensures  IsValidDistributedSystemTraceAndBehavior(trace', db');
+        ensures  DistributedSystemBehaviorRefinesSpec(db')
+                 ==> exists sb :: DistributedSystemBehaviorRefinesSpecBehaviorWithNonPivotsAsStutters(db, sb, indices, pivot_index);
+        ensures  entry_pos <= |trace'| < |trace|;
+        ensures  trace'[..entry_pos] == trace[..entry_pos];
+        decreases |group| - in_position_right + in_position_left, 0;
+    {
+        var actor := GetEntryActor(group[0]);
+
+        var begin_entry_pos := indices[pivot_index] - pivot_index;
+        var end_entry_pos := indices[pivot_index] + |group| - pivot_index - 1;
+
+        lemma_PerformReductionOfSpecificIndicesHelper5(trace, min_level, mid_level, max_level, entry_pos, indices, group, pivot_index, begin_entry_pos, end_entry_pos);
+        lemma_PerformReductionOfSpecificIndicesHelper6(trace, min_level, mid_level, max_level, group, actor, begin_entry_pos, end_entry_pos);
+        lemma_PerformReductionOfSpecificIndicesHelper7(trace, min_level, mid_level, max_level, group, actor, begin_entry_pos, end_entry_pos);
+        assert trace[begin_entry_pos..begin_entry_pos+|group|] == group;
+        trace', db' := lemma_PerformOneReductionStep(trace, db, actor, min_level, begin_entry_pos, end_entry_pos, pivot_index);
+        var trace'' := lemma_ReductionPreservesTraceValid(trace, min_level, mid_level, max_level, begin_entry_pos, |group|);
+        assert trace' == trace'';
+        if DistributedSystemBehaviorRefinesSpec(db') {
+            var sb :|    DistributedSystemBehaviorRefinesSpecBehavior(db, sb) &&
+                      forall i :: begin_entry_pos <= i <= end_entry_pos && i != begin_entry_pos + pivot_index ==> sb[i] == sb[i+1];
+            assert DistributedSystemBehaviorRefinesSpecBehaviorWithNonPivotsAsStutters(db, sb, indices, pivot_index);
+        }
+    }
+
     lemma lemma_PerformReductionOfSpecificIndices(
         trace:Trace,
         db:seq<DistributedSystemState>,
@@ -215,17 +727,17 @@ module Reduction3Module
         requires TraceValid(trace, min_level, max_level);
         requires |indices| == |group| > 0;
         requires 0 <= entry_pos <= indices[0];
-        requires forall i, j {:trigger indices[i] < indices[j]}{:trigger indices[i] <= indices[j]}{:trigger indices[j] > indices[i]}{:trigger indices[j] >= indices[i]} :: 0 <= i < j < |indices| ==> indices[i] < indices[j];
+        requires forall i, j {:trigger indices[i], indices[j]} :: 0 <= i < j < |indices| ==> indices[i] < indices[j];
         requires forall i :: 0 <= i < |indices| ==> 0 <= indices[i] < |trace| && trace[indices[i]] == group[i];
         requires min_level < mid_level <= max_level;
         requires EntryGroupValidForLevels(group, min_level, mid_level);
         requires GetEntryLevel(group[0]) == min_level;
         requires pivot_index == last(group).pivot_index;
         requires forall i :: 0 <= i < |group| ==> GetEntryActor(group[i]) == GetEntryActor(group[0]);   // All for the same actor
-        requires forall group_index, trace_index {:trigger indices[group_index] < trace_index, trace_index < indices[group_index+1]} ::
-                                                    0 <= group_index < |indices| - 1 
-                                                 && indices[group_index] < trace_index < indices[group_index+1] 
-                                                 ==> GetEntryActor(trace[trace_index]) != GetEntryActor(group[0]);
+        requires forall i, trace_index {:trigger indices[i], trace[trace_index], indices[i+1]} ::
+                                      0 <= i < |indices| - 1
+                                   && indices[i] < trace_index < indices[i+1]
+                                   ==> GetEntryActor(trace[trace_index]) != GetEntryActor(group[0]);
         requires 0 <= in_position_left <= pivot_index <= in_position_right < |group|;
         requires forall k :: in_position_left <= k <= in_position_right ==> k - pivot_index == indices[k] - indices[pivot_index];
 
@@ -235,34 +747,19 @@ module Reduction3Module
                  ==> exists sb :: DistributedSystemBehaviorRefinesSpecBehaviorWithNonPivotsAsStutters(db, sb, indices, pivot_index);
         ensures  entry_pos <= |trace'| < |trace|;
         ensures  trace'[..entry_pos] == trace[..entry_pos];
-        decreases |group| - in_position_right + in_position_left;
+        decreases |group| - in_position_right + in_position_left, 1;
     {
         var actor := GetEntryActor(group[0]);
 
         if in_position_left > 0 {
-            var trace_mid, db_mid, indices_mid := lemma_MoveRightMoverIntoPlace(trace, db, min_level, mid_level, max_level, entry_pos, indices, group, pivot_index, in_position_left, in_position_right);
-            trace', db' := lemma_PerformReductionOfSpecificIndices(trace_mid, db_mid, min_level, mid_level, max_level, entry_pos, indices_mid, group, pivot_index, in_position_left - 1, in_position_right);
+            trace', db' := lemma_PerformReductionOfSpecificIndicesCase1(trace, db, min_level, mid_level, max_level, entry_pos, indices, group, pivot_index, in_position_left, in_position_right);
         }
         else if in_position_right < |indices| - 1 {
-            var trace_mid, db_mid, indices_mid := lemma_MoveLeftMoverIntoPlace(trace, db, min_level, mid_level, max_level, entry_pos, indices, group, pivot_index, in_position_left, in_position_right);
-            trace', db' := lemma_PerformReductionOfSpecificIndices(trace_mid, db_mid, min_level, mid_level, max_level, entry_pos, indices_mid, group, pivot_index, in_position_left, in_position_right + 1);
+            trace', db' := lemma_PerformReductionOfSpecificIndicesCase2(trace, db, min_level, mid_level, max_level, entry_pos, indices, group, pivot_index, in_position_left, in_position_right);
         }
         else {
             assert in_position_left == 0 && in_position_right == |indices| - 1;
-            var begin_entry_pos := indices[pivot_index] - pivot_index;
-            var end_entry_pos := indices[pivot_index] + |group| - pivot_index - 1;
-
-            lemma_PerformReductionOfSpecificIndicesHelper1(trace, min_level, mid_level, max_level, entry_pos, indices, group, pivot_index, begin_entry_pos, end_entry_pos);
-            lemma_PerformReductionOfSpecificIndicesHelper2(trace, min_level, mid_level, max_level, group, actor, begin_entry_pos, end_entry_pos);
-            lemma_PerformReductionOfSpecificIndicesHelper3(trace, min_level, mid_level, max_level, group, actor, begin_entry_pos, end_entry_pos);
-            trace', db' := lemma_PerformOneReductionStep(trace, db, actor, min_level, begin_entry_pos, end_entry_pos, pivot_index);
-            var trace'' := lemma_ReductionPreservesTraceValid(trace, min_level, mid_level, max_level, begin_entry_pos, |group|);
-            assert trace' == trace'';
-            if DistributedSystemBehaviorRefinesSpec(db') {
-                var sb :|    DistributedSystemBehaviorRefinesSpecBehavior(db, sb) &&
-                          forall i :: begin_entry_pos <= i <= end_entry_pos && i != begin_entry_pos + pivot_index ==> sb[i] == sb[i+1];
-                assert DistributedSystemBehaviorRefinesSpecBehaviorWithNonPivotsAsStutters(db, sb, indices, pivot_index);
-            }
+            trace', db' := lemma_PerformReductionOfSpecificIndicesCase3(trace, db, min_level, mid_level, max_level, entry_pos, indices, group, pivot_index, in_position_left, in_position_right);
         }
     }
 
@@ -283,16 +780,16 @@ module Reduction3Module
         requires TraceValid(trace, min_level, max_level);
         requires |indices| == |group| > 0;
         requires 0 <= entry_pos <= indices[0];
-        requires forall i, j {:trigger indices[i] < indices[j]}{:trigger indices[i] <= indices[j]}{:trigger indices[j] > indices[i]}{:trigger indices[j] >= indices[i]} :: 0 <= i < j < |indices| ==> indices[i] < indices[j];
+        requires forall i, j {:trigger indices[i], indices[j]} :: 0 <= i < j < |indices| ==> indices[i] < indices[j];
         requires forall i :: 0 <= i < |indices| ==> 0 <= indices[i] < |trace| && trace[indices[i]] == group[i];
         requires min_level < mid_level <= max_level;
         requires EntryGroupValidForLevels(group, min_level, mid_level);
         requires GetEntryLevel(group[0]) == min_level;
         requires forall i :: 0 <= i < |group| ==> GetEntryActor(group[i]) == GetEntryActor(group[0]);   // All for the same actor
-        requires forall group_index, trace_index {:trigger indices[group_index] < trace_index, trace_index < indices[group_index+1]} ::
-                                                    0 <= group_index < |indices| - 1 
-                                                 && indices[group_index] < trace_index < indices[group_index+1] 
-                                                 ==> GetEntryActor(trace[trace_index]) != GetEntryActor(group[0]);
+        requires forall i, trace_index {:trigger indices[i], trace[trace_index], indices[i+1]} ::
+                                      0 <= i < |indices| - 1
+                                   && indices[i] < trace_index < indices[i+1]
+                                   ==> GetEntryActor(trace[trace_index]) != GetEntryActor(group[0]);
 
         ensures  TraceValid(trace', min_level, max_level);
         ensures  IsValidDistributedSystemTraceAndBehavior(trace', db');
